Prove wfness of SimpleVSTLC too

src/named/SimpleVSTLC.v
@@ -1,24 +1,19 @@
-
-Require Import mathcomp.ssreflect.all_ssreflect.
 Set Implicit Arguments.
-Unset Strict Implicit.
-Unset Printing Implicit Defensive.
 Set Bullet Behavior "Strict Subproofs".
 
-
-From Ltac2 Require Import Ltac2.
-Set Default Proof Mode "Classic".
+Require Import String List.
+Import ListNotations.
+Open Scope string.
+Open Scope list.
 From Utils Require Import Utils.
-From Named Require Import Exp ARule.
-From Named Require Import ImCore Pf.
-From Named Require Import SimpleVSubst.
-Import Exp.Notations ARule.Notations.
-Require Import String.
+From Named Require Import Core Elab SimpleVSubst.
+Import Core.Notations.
 
-Set Default Proof Mode "Classic".
+Require Coq.derive.Derive.
+
 
 Definition stlc :=
-  [::[:> "G" : #"env", "A" : #"ty", "B" : #"ty",
+  [[:> "G" : #"env", "A" : #"ty", "B" : #"ty",
       "e" : #"el" (#"ext" %"G" %"A") %"B",
       "G'" : #"env",
       "g" : #"sub" %"G'" %"G"
@@ -67,184 +62,13 @@ Definition stlc :=
       #"->" "t" "t'" : #"ty"
   ]]%arule++subst_lang.
 
-Import OptionMonad.
-Definition simple_subst_to_pf_ty (e:exp) : option pf :=
-  match e with
-  | var x => Some (pvar x)
-  | con "->" [:: B; A] =>
-    do pA <- simple_subst_to_pf_ty A;
-       pB <- simple_subst_to_pf_ty B;
-       ret (pcon "->" [:: pB; pA])
-  | _ => None
-  end.
 
-
-Fixpoint simple_subst_to_pf_env (e:exp) : option pf :=
-  match e with
-  | var x => Some (pvar x)
-  | con "emp" [::] => Some (pcon "emp" [::])
-  | con "ext" [:: A; G] =>
-    do pa <- simple_subst_to_pf_ty A;
-       pG <- simple_subst_to_pf_env G;
-       ret (pcon "ext" [:: pa; pG])
-  | _ => None
-  end.
-
-Definition simple_subst_to_pf_sort (t:sort) : option pf :=
-  match t with
-  | scon "env" [::] => Some (pcon "env" [::])
-  | scon "ty" [::] => Some (pcon "ty" [::])
-  | scon "sub" [:: G'; G] =>
-    do pG' <- simple_subst_to_pf_env G';
-       pG <- simple_subst_to_pf_env G;
-       ret (pcon "sub" [:: pG'; pG])
-  | scon "el" [:: A; G] =>
-    do pa <- simple_subst_to_pf_ty A;
-       pG <- simple_subst_to_pf_env G;
-       ret (pcon "el" [:: pa; pG])
-  | scon "val" [:: A; G] =>
-    do pa <- simple_subst_to_pf_ty A;
-       pG <- simple_subst_to_pf_env G;
-       ret (pcon "val" [:: pa; pG])
-  | _ => None
-  end.
-
-
-Fixpoint simple_subst_to_pf_sub (c : pf_ctx) (e :exp) G_l : option (pf * pf) :=
-  match e with
-  | var x =>
-    do (pcon "sub" [:: G_r;_]) <- named_list_lookup_err c x;
-       ret (pvar x, G_r)
-  | con "id" [::] =>
-    do ret (pcon "id" [:: G_l], G_l)
-  | con "cmp" [:: g; f] =>
-    do (p_f,G_fr) <- simple_subst_to_pf_sub c f G_l;
-       (p_g, G_gr) <- simple_subst_to_pf_sub c g G_fr;
-       ret (pcon "cmp" [:: p_g; p_f; G_gr; G_fr; G_l], G_gr)
-  | con "forget" [::] =>
-    do ret (pcon "forget" [:: G_l], pcon "emp" [::])
-  | con "snoc" [:: e; f] =>
-    do (p_f,G_fr) <- simple_subst_to_pf_sub c f G_l;
-       (p_e, pA) <- simple_subst_to_pf_val c e G_l;
-       ret (pcon "snoc" [:: p_e; p_f; pA; G_fr; G_l], pcon "ext" [:: pA; G_fr])
-  | con "wkn" [::] =>
-    do (pcon "ext" [:: A; G]) <- Some G_l;
-       ret (pcon "wkn" [:: A; G], G)
-  | _ => None
-  end
-with simple_subst_to_pf_val c e G : option (pf * pf) :=
-       match e with
-       | var x =>
-         do (pcon "val" [:: A; _]) <- named_list_lookup_err c x;
-         ret (pvar x, A)
-       | con "val_subst" [:: e; f] =>
-         do (p_f,G_fr) <- simple_subst_to_pf_sub c f G;
-            (p_e, pA) <- simple_subst_to_pf_val c e G_fr;
-            ret (pcon "val_subst" [:: p_e; pA; p_f; G_fr; G], pA)
-      | con "hd" [::] =>
-        do (pcon "ext" [:: A; G]) <- Some G;
-           ret (pcon "hd" [:: A; G], A)
-       | con "lambda" [:: e; A] =>
-         do pA <- simple_subst_to_pf_ty A;
-            (p_e, pB) <- simple_subst_to_pf_el c e (pcon "ext" [:: pA; G]);
-            ret (pcon "lambda" [:: p_e; pB; pA; G], pcon "->" [:: pB; pA])
-       | _ => None
-       end
-with simple_subst_to_pf_el c e G : option (pf * pf) :=
-       match e with
-       | var x =>
-         do (pcon "el" [:: A; _]) <- named_list_lookup_err c x;
-         ret (pvar x, A)
-       | con "el_subst" [:: e; f] =>
-         do (p_f,G_fr) <- simple_subst_to_pf_sub c f G;
-            (p_e, pA) <- simple_subst_to_pf_el c e G_fr;
-            ret (pcon "el_subst" [:: p_e; pA; p_f; G_fr; G], pA)
-      | con "ret" [:: v] =>
-        do (pv,A) <- simple_subst_to_pf_val c v G;
-           ret (pcon "ret" [:: pv; A; G], A)
-       | con "app" [:: e'; e] =>
-         do (p_e, pcon "->" [:: pB; pA]) <- simple_subst_to_pf_el c e G;
-            (p_e', _) <- simple_subst_to_pf_el c e' G;
-            ret (pcon "app" [:: p_e'; p_e; pB; pA; G], pB)
-       | _ => None
-end.
-
-Definition simple_subst_to_pf_term (c : pf_ctx) (e :exp) t : option pf :=
-  match t with
-  | pcon "env" [::] => simple_subst_to_pf_env e
-  | pcon "ty" [::] => simple_subst_to_pf_ty e
-  | pcon "sub" [:: _ ; G_l] =>
-    do (p,_) <- simple_subst_to_pf_sub c e G_l;
-       ret p
-  | pcon "el" [:: _ ; G] =>
-    do (p,_) <- simple_subst_to_pf_el c e G;
-       ret p
-  | pcon "val" [:: _ ; G] =>
-    do (p,_) <- simple_subst_to_pf_val c e G;
-       ret p
-  | _ => None
-  end.
-
-Fixpoint simple_subst_to_pf_ctx (c : ctx) : option pf_ctx :=
-  match c with
-  | [::] => do ret [::]
-  | (n,t)::c' =>
-    do pc' <- simple_subst_to_pf_ctx c';
-       pt <- simple_subst_to_pf_sort t;
-       ret (n,pt)::pc'
-  end.
-
-Definition simple_subst_to_pf_rule (r : rule) : option rule_pf :=
-  match r with
-  | sort_rule c args =>
-    do pc <- simple_subst_to_pf_ctx c;
-    ret sort_rule_pf pc args
-  | term_rule c args t =>
-    do pt <- simple_subst_to_pf_sort t;
-       pc <- simple_subst_to_pf_ctx c;
-    ret term_rule_pf pc args pt
-  | sort_le c t1 t2 =>
-    do pt1 <- simple_subst_to_pf_sort t1;
-       pt2 <- simple_subst_to_pf_sort t2;
-       pc <- simple_subst_to_pf_ctx c;
-    ret sort_le_pf pc pt1 pt2
-  | term_le c e1 e2 t =>
-    do pt <- simple_subst_to_pf_sort t;
-       pc <- simple_subst_to_pf_ctx c;
-       pe1 <- simple_subst_to_pf_term pc e1 pt;
-       pe2 <- simple_subst_to_pf_term pc e2 pt;
-    ret term_le_pf pc pe1 pe2 pt
-end.
-
-Fixpoint simple_subst_to_pf_lang (l : lang) : option pf_lang :=
-  match l with
-  | [::] => do ret [::]
-  | (n,r)::l' =>
-    do pl' <- simple_subst_to_pf_lang l';
-       pr <- simple_subst_to_pf_rule r;
-       ret (n,pr)::pl'
-  end.
-
-
-Definition vstlc_elab :=
-  Eval compute in
-  match simple_subst_to_pf_lang stlc with
-  | Some l => l
-  | None => [::]
-  end.
-Goal match vsubst_elab with [::] => False | _ => True end.
-    by compute.
-Qed.
-
-
-Lemma simple_stlc_wf : wf_lang stlc.
+Derive stlc_elab
+       SuchThat (elab_lang stlc stlc_elab)
+       As stlc_wf.
 Proof.
-  prove_wf_with_fn simple_subst_to_pf_lang.
+  auto_elab.
+  Unshelve.
+  all: cleanup_auto_elab.
 Qed.
 
-Derive elab_stlc
-       SuchThat (Some elab_stlc = simple_subst_to_pf_lang stlc)
-  As elab_stlc_pf.
-Proof.
-  compute; reflexivity.
-Qed.
